wip: generalizing pwp

lawyer/nonblocking/pwp.v
@@ -30,25 +30,28 @@ Definition phys_SI {Λ} (LG: LangEM Λ) `{invGS_gen HasNoLc Σ} {lG: lgem_GS Σ}
 
 (** not turning these into instances to avoid incorrect Iris instantiations *)
 
-Definition irisG_looping {Λ} (LG: LangEM Λ) `{invGS_gen HasNoLc Σ} {lG: lgem_GS Σ}:
+Definition irisG_looping {Λ} (LG: LangEM Λ) `{invGS_gen HasNoLc Σ} {lG: lgem_GS Σ}
+  (si_add: execution_trace Λ -> iProp Σ):
   irisG Λ LoopingModel Σ := {|
-    state_interp := phys_SI LG (lG := lG);
+    state_interp etr mtr := (phys_SI LG (lG := lG) etr mtr ∗ si_add etr)%I;
     fork_post := fun _ _ => (⌜ True ⌝)%I;
 |}. 
 
-(* TODO: rename *)
-Definition iris_OM_into_Looping {Σ} `(Hinv : @IEMGS Λ M LG EM Σ):
+
+Definition IEMGS_into_Looping {Σ} `(Hinv : @IEMGS Λ M LG EM Σ) 
+  (si_add: execution_trace Λ -> iProp Σ):
   irisG Λ LoopingModel Σ.
 Proof using.
-  eapply irisG_looping; apply Hinv.  
+  eapply (@irisG_looping _ _ _ _ _ si_add).
+  Unshelve. apply Hinv.
 Defined.
-
 
 Definition looping_trace: auxiliary_trace LoopingModel :=
   trace_singleton ().
 
 
 Lemma pwp_MU_ctx_take_step {Σ} `{Hinv : @IEMGS heap_lang M HeapLangEM EM Σ}
+  si_add
     s Φ ex atr tp1 K e1 tp2 σ1 e2 σ2 efs ζ P:
     let (E1, E2) := (ectx_fill K e1, ectx_fill K e2) in
     valid_exec ex →
@@ -56,40 +59,40 @@ Lemma pwp_MU_ctx_take_step {Σ} `{Hinv : @IEMGS heap_lang M HeapLangEM EM Σ}
     trace_ends_in ex (tp1 ++ E1 :: tp2, σ1) →
     locale_of tp1 E1 = ζ ->
     state_interp ex atr -∗
+    si_add ex -∗
     (let hGS: @heapGS Σ M EM := {| heap_iemgs := Hinv |} in
      let oτ' := step_fork (trace_last ex) (tp1 ++ E2 :: tp2 ++ efs, σ2) in
      @MU_impl _ EM Σ hGS oτ' ⊤ ζ P ) -∗
-    (let _ := iris_OM_into_Looping in pwp s ⊤ ζ e1 Φ)
+    (let _ := IEMGS_into_Looping Hinv si_add in pwp s ⊤ ζ e1 Φ)
     ={⊤,∅}=∗   |={∅}▷=>^(S $ trace_length ex)   |={∅,⊤}=>
     ∃ δ' ℓ,
-      state_interp (trace_extend ex (Some ζ) (tp1 ++ E2 :: tp2 ++ efs, σ2))
-                   (trace_extend atr ℓ δ') ∗
-      (let _ := iris_OM_into_Looping in pwp s ⊤ ζ e2 Φ) ∗ 
+      let etr' := trace_extend ex (Some ζ) (tp1 ++ E2 :: tp2 ++ efs, σ2) in
+      state_interp etr' (trace_extend atr ℓ δ') ∗
+      si_add etr' ∗
+      (let _ := IEMGS_into_Looping Hinv si_add in pwp s ⊤ ζ e2 Φ) ∗ 
       ([∗ list] i↦ef ∈ efs,
         let τf := locale_of (tp1 ++ E1 :: tp2 ++ take i efs) ef in
-        (let _ := iris_OM_into_Looping in pwp s ⊤ τf ef
-                                            (fork_post τf) (* for pwp *)
-                                            (* (let _: ObligationsGS Σ := @iem_fairnessGS _ _ _ _ _ Hinv in *)
-                                            (*   fun _ => obls τf ∅) *)
-        )
+        (let _ := IEMGS_into_Looping Hinv si_add in
+         pwp s ⊤ τf ef (fork_post τf) (* for pwp *)        )
       ) ∗
       P.
 Proof using.
   simpl.
-  iIntros (Hex Hstp Hei Hlocale) "HSI MU Hwp".
+  iIntros (Hex Hstp Hei Hlocale) "HSI ADD MU Hwp".
   rewrite /pwp. 
   rewrite wp_unfold /wp_pre.
   destruct (to_val e1) eqn:He1.
   { erewrite val_stuck in He1; done. }
   simpl. 
   iDestruct "HSI" as "(%EV & PHYS & MSI)". simpl. 
-  iMod ("Hwp" $! _ looping_trace K with "[//] [] [] PHYS") as "[Hs Hwp]".
+  iMod ("Hwp" $! _ looping_trace K with "[//] [] [] [PHYS ADD]") as "[Hs Hwp]".
   1, 2: done.
+  { iFrame. }
   iDestruct ("Hwp" with "[]") as "Hwp"; first done.
   iModIntro. 
   iApply (step_fupdN_wand with "Hwp").
   iIntros "!> Hwp".
-  iMod "Hwp" as ([] []) "(PHYS & WP & WPS')".
+  iMod "Hwp" as ([] []) "((PHYS & ADD) & WP & WPS')".
   
   rewrite /MU /MU_impl. iMod ("MU" $! (trace_extend _ _ (_, _)) with "[PHYS MSI]") as (δ ρ) "TI".
   { rewrite /trace_interp_interim.
@@ -108,17 +111,23 @@ Proof using.
 Qed.
 
 
+Definition si_add_none {Λ} {Σ} (etr: execution_trace Λ): iProp Σ := emp%I. 
+
+(* TODO: move? *)
+Definition IEMGS_into_Looping_simpl {Σ} `(Hinv : @IEMGS Λ M LG EM Σ) :=
+  IEMGS_into_Looping Hinv si_add_none. 
+
 (* TODO: move? try to unify with sswp_MU_wp_fupd  *)
 Lemma sswp_pwp_fupd {Σ} {iG: invGS_gen HasNoLc Σ} {hG: heap1GS Σ}
   s E E' τ e Φ
   (NVAL: language.to_val e = None):
-  let iG := irisG_looping HeapLangEM (lG := hG) in 
+  let iG := irisG_looping HeapLangEM si_add_none (lG := hG) in 
   (|={E,E'}=> sswp s E' e (λ e', ▷ |={E',E}=> pwp s E τ e' Φ)%I) -∗
     pwp s E τ e Φ.
 Proof using.
   rewrite /pwp wp_unfold /wp_pre.
   iIntros "Hsswp". rewrite NVAL. 
-  iIntros (extr atr K tp1 tp2 σ1 Hvalid Hζ Hextr) "Hσ".
+  iIntros (extr atr K tp1 tp2 σ1 Hvalid Hζ Hextr) "(Hσ & ADD)".
   iMod "Hsswp" as "foo".
   rewrite /sswp. rewrite NVAL.
   iSimpl in "Hσ".
@@ -142,7 +151,7 @@ Qed.
 Lemma sswp_pwp {Σ} {iG: invGS_gen HasNoLc Σ} {hG: heap1GS Σ}
   s E τ e Φ
   (NVAL: language.to_val e = None):
-  let iG := irisG_looping HeapLangEM (lG := hG) in 
+  let iG := irisG_looping HeapLangEM si_add_none (lG := hG) in 
   sswp s E e (λ e', ▷ pwp s E τ e' Φ)%I -∗
   pwp s E τ e Φ.
 Proof using.
@@ -155,11 +164,12 @@ Qed.
 Lemma pre_step_looping_wfree_elim {Σ M} {EM: ExecutionModel heap_lang M}
   {Hinv : @IEMGS _ _ HeapLangEM EM Σ}
   (P: iProp Σ):
-  (let _ := iris_OM_into_Looping (EM := EM) in |~~| P) -∗ (|~~| P).
+  (let _ := IEMGS_into_Looping Hinv si_add_none (EM := EM) in |~~| P) -∗ (|~~| P).
 Proof using.
   simpl. iIntros "P".
   rewrite !weakestpre.pre_step_unseal. rewrite /pre_step_def. simpl. 
   iIntros (etr atr) "(%EVOL & PHYS & MSI)". simpl.
-  iMod ("P" $! etr looping_trace with "PHYS") as "(PHYS & P)".
+  iMod ("P" $! etr looping_trace with "[PHYS]") as "((PHYS & ADD) & P)".
+  { iFrame. }
   iModIntro. by iFrame.
 Qed.
