lawyer/nonblocking/logrel/logrel.v
@@ -38,7 +38,7 @@ Section logrel.
 
   Program Definition interp_arrow : D -n> D :=
     λne ii, PersPred (λ w, □ ∀ τ v, ▷ ii v →
-      let _ := irisG_looping HeapLangEM (lG := hG) in 
+      let _ := irisG_looping HeapLangEM si_add_none (lG := hG) in 
       pwp MaybeStuck ⊤ τ (App (of_val w) (of_val v)) ii )%I.
   Solve Obligations with solve_proper.
   Instance interp_arrow_contractive : Contractive interp_arrow.
@@ -110,7 +110,7 @@ Section logrel.
   Proof. rewrite /interp; apply fixpoint_unfold. Qed.
 
   Definition interp_expr (τ: locale heap_lang) (e: expr heap_lang) : iProp Σ :=
-    let _ := irisG_looping HeapLangEM (lG := hG) in 
+    let _ := irisG_looping HeapLangEM si_add_none (lG := hG) in 
     pwp MaybeStuck ⊤ τ e interp.
 
   Definition interp_env (vs : gmap string (val heap_lang)) : iProp Σ :=
